interface for hyperstack complete

ulib/FStar.Monotonic.HyperStack.fst
@@ -92,7 +92,9 @@ private let lemma_pop_is_popped (m0:mem{poppable m0})
 
 let modifies_drop_tip _ _ _ _ = ()
 
-let eternal_disjoint_from_tip h r = ()
+let eternal_disjoint_from_tip _ _ = ()
+
+let above_tip_is_live #_ #_ _ _ = ()
 
 let lemma_heap_equality_cancel_same_mref_upd #_ #_ h r x y =
   let h0 = upd (upd h r x) r y in
@@ -111,14 +113,12 @@ let lemma_heap_equality_commute_distinct_upds #_ #_ #_ #_ h r1 r2 x y =
   if frameOf r1 = frameOf r2 then Heap.lemma_heap_equality_commute_distinct_upds (Map.sel h.h (frameOf r1)) (as_ref r1) (as_ref r2) x y;
   assert (Map.equal h0.h h1.h)
 
-let lemma_next_addr_contained_refs_addr ()
-  :Lemma (forall (a:Type0) (rel:preorder a) (r:mreference a rel) (m:mem).
-            m `contains` r ==> as_addr r < Heap.next_addr (get_hmap m `Map.sel` frameOf r))
-  = let aux (a:Type0) (rel:preorder a) (r:mreference a rel) (m:mem)
-      :Lemma (m `contains` r ==> as_addr r < Heap.next_addr (get_hmap m `Map.sel` frameOf r))
-      = Heap.lemma_next_addr_contained_refs_addr (get_hmap m `Map.sel` frameOf r) (as_ref r)
-    in
-    Classical.forall_intro_4 aux
+let lemma_next_addr_contained_refs_addr _ =
+  let aux (a:Type0) (rel:preorder a) (r:mreference a rel) (m:mem)
+    :Lemma (m `contains` r ==> as_addr r < Heap.next_addr (get_hmap m `Map.sel` frameOf r))
+    = Heap.lemma_next_addr_contained_refs_addr (get_hmap m `Map.sel` frameOf r) (as_ref r)
+  in
+  Classical.forall_intro_4 aux
 
 private let lemma_upd_1 #a #rel (h:mem) (x:mreference a rel) (v:a{rel (sel h x) v}) : Lemma
   (requires (contains h x))
@@ -142,249 +142,67 @@ private val lemma_live_1: #a:Type ->  #a':Type -> #rel:preorder a -> #rel':preor
   (ensures  (frameOf x <> frameOf x' \/ ~ (as_ref x === as_ref x')))
 let lemma_live_1 #a #a' #rel #rel' h x x' = ()
 
-let above_tip_is_live (#a:Type) (#rel:preorder a) (m:mem) (x:mreference a rel) : Lemma
-  (requires (frameOf x `is_above` get_tip m))
-  (ensures (frameOf x `is_in` get_hmap m))
-  = ()
-
-
 (*** Untyped views of references *)
 
 (* Definition and ghost decidable equality *)
 
-noeq abstract type aref: Type0 =
-| ARef:
-    (aref_region: rid) ->
-    (aref_aref: Heap.aref) ->
-    aref
+noeq type aref =
+  | ARef: aref_region:rid ->
+          aref_aref:Heap.aref ->
+          aref
 
-abstract let dummy_aref : aref = ARef root Heap.dummy_aref
+let dummy_aref = ARef root Heap.dummy_aref
 
-abstract let aref_equal
-  (a1 a2: aref)
-: Ghost bool
-  (requires True)
-  (ensures (fun b -> b == true <==> a1 == a2))
-= a1.aref_region = a2.aref_region && Heap.aref_equal a1.aref_aref a2.aref_aref
+let aref_equal a1 a2 = a1.aref_region = a2.aref_region && Heap.aref_equal a1.aref_aref a2.aref_aref
 
-(* Introduction rule *)
+let aref_of #_ #_ r = ARef (frameOf r) (Heap.aref_of (as_ref r))
 
-abstract let aref_of
-  (#t: Type)
-  (#rel: preorder t)
-  (r: mreference t rel)
-  : Tot aref
-  = ARef (frameOf r) (Heap.aref_of (as_ref r))
+let frameOf_aref a = a.aref_region
 
-(* Operators lifted from reference *)
+let frameOf_aref_of #_ #_ _ = ()
 
-abstract let frameOf_aref
-  (a: aref)
-: GTot rid
-= a.aref_region
+let aref_as_addr a = Heap.addr_of_aref a.aref_aref
 
-abstract let frameOf_aref_of
-  (#t: Type)
-  (#rel: preorder t)
-  (r: mreference t rel)
-: Lemma
-  (frameOf_aref (aref_of r) == frameOf r)
-  [SMTPat (frameOf_aref (aref_of r))]
-= ()
+let aref_as_addr_aref_of #_ #_ r = Heap.addr_of_aref_of (as_ref r)
 
-abstract let aref_as_addr
-  (a: aref)
-: GTot (x: nat { x > 0 } )
-= Heap.addr_of_aref a.aref_aref
+let aref_is_mm r = Heap.aref_is_mm r.aref_aref
 
-abstract let aref_as_addr_aref_of
-  (#t: Type)
-  (#rel: preorder t)
-  (r: mreference t rel)
-: Lemma
-  (aref_as_addr (aref_of r) == as_addr r)
-  [SMTPat (aref_as_addr (aref_of r))]
-= Heap.addr_of_aref_of (as_ref r)
+let is_mm_aref_of #_ #_ r = Heap.is_mm_aref_of (as_ref r)
 
-abstract let aref_is_mm
-  (r: aref)
-: GTot bool
-= Heap.aref_is_mm r.aref_aref
-
-abstract let is_mm_aref_of
-  (#t: Type)
-  (#rel: preorder t)
-  (r: mreference t rel)
-: Lemma
-  (aref_is_mm (aref_of r) == is_mm r)
-  [SMTPat (aref_is_mm (aref_of r))]
-= Heap.is_mm_aref_of (as_ref r)
-
-abstract let aref_unused_in
-  (a: aref)
-  (h: mem)
-: GTot Type0
-= ~ (live_region h a.aref_region) \/
+let aref_unused_in a h =
+  ~ (live_region h a.aref_region) \/
   Heap.aref_unused_in a.aref_aref (Map.sel h.h a.aref_region)
 
-abstract let unused_in_aref_of
-  (#t: Type)
-  (#rel: preorder t)
-  (r: mreference t rel)
-  (h: mem)
-: Lemma
-  (aref_unused_in (aref_of r) h <==> unused_in r h)
-  [SMTPat (aref_unused_in (aref_of r) h)]
-= Heap.unused_in_aref_of (as_ref r) (Map.sel h.h (frameOf r))
+let unused_in_aref_of #_ #_ r h = Heap.unused_in_aref_of (as_ref r) (Map.sel h.h (frameOf r))
 
-abstract
-val contains_aref_unused_in: #a:Type -> #rel: preorder a -> h:mem -> x:mreference a rel -> y:aref -> Lemma
-  (requires (contains h x /\ aref_unused_in y h))
-  (ensures  (frameOf x <> frameOf_aref y \/ as_addr x <> aref_as_addr y))
-  [SMTPat (contains h x); SMTPat (aref_unused_in y h)]
-let contains_aref_unused_in #a #rel h x y =
+let contains_aref_unused_in #_ #_ h x y =
   if frameOf x = frameOf_aref y
   then
     Heap.contains_aref_unused_in (Map.sel h.h (frameOf x)) (as_ref x) y.aref_aref
   else ()
 
-(* Elimination rule *)
+let aref_live_at h a v rel =
+  live_region h a.aref_region /\
+  Heap.aref_live_at (Map.sel h.h a.aref_region) a.aref_aref v rel
 
-abstract
-let aref_live_at
-  (h: mem)
-  (a: aref)
-  (v: Type)
-  (rel: preorder v)
-: GTot Type0
-= live_region h a.aref_region
-  /\ Heap.aref_live_at (Map.sel h.h a.aref_region) a.aref_aref v rel
+let greference_of a v rel = MkRef a.aref_region (Heap.gref_of a.aref_aref v rel)
 
-abstract
-let greference_of
-  (a: aref)
-  (v: Type)
-  (rel: preorder v)
-: Ghost (mreference v rel)
-  (requires (exists h . aref_live_at h a v rel))
-  (ensures (fun _ -> True))
-= MkRef a.aref_region (Heap.gref_of a.aref_aref v rel)
+let reference_of h a v rel = MkRef a.aref_region (Heap.ref_of (Map.sel h.h a.aref_region) a.aref_aref v rel)
 
-abstract
-let reference_of
-  (h: mem)
-  (a: aref)
-  (v: Type)
-  (rel: preorder v)
-: Pure (mreference v rel)
-  (requires (aref_live_at h a v rel))
-  (ensures (fun x -> aref_live_at h a v rel /\ frameOf x == frameOf_aref a /\ as_addr x == aref_as_addr a /\ is_mm x == aref_is_mm a))
-= MkRef a.aref_region (Heap.ref_of (Map.sel h.h a.aref_region) a.aref_aref v rel)
+let aref_live_at_aref_of _ #_ #_ _ = ()
 
-abstract
-let aref_live_at_aref_of
-  (h: mem)
-  (#t: Type0)
-  (#rel: preorder t)
-  (r: mreference t rel)
-: Lemma
-  (aref_live_at h (aref_of r) t rel <==> contains h r)
-  [SMTPat (aref_live_at h (aref_of r) t rel)]
-= ()
+let contains_greference_of _ _ _ _ = ()
 
-abstract
-let contains_greference_of
-  (h: mem)
-  (a: aref)
-  (t: Type0)
-  (rel: preorder t)
-: Lemma
-  (requires (exists h' . aref_live_at h' a t rel))
-  (ensures ((exists h' . aref_live_at h' a t rel) /\ (contains h (greference_of a t rel) <==> aref_live_at h a t rel)))
-  [SMTPatOr [
-    [SMTPat (contains h (greference_of a t rel))];
-    [SMTPat (aref_live_at h a t rel)];
-  ]]
-= ()
+let aref_of_greference_of _ _ _ = ()
 
-abstract
-let aref_of_greference_of
-  (a: aref)
-  (v: Type0)
-  (rel: preorder v)
-: Lemma
-  (requires (exists h' . aref_live_at h' a v rel))
-  (ensures ((exists h' . aref_live_at h' a v rel) /\ aref_of (greference_of a v rel) == a))
-  [SMTPat (aref_of (greference_of a v rel))]
-= ()
+let frameOf_greference_of _ _ _ = ()
 
-(* Operators lowered to rref *)
+let as_addr_greference_of _ _ _ = ()
 
-abstract let frameOf_greference_of
-  (a: aref)
-  (t: Type)
-  (rel: preorder t)
-: Lemma
-  (requires (exists h . aref_live_at h a t rel))
-  (ensures ((exists h . aref_live_at h a t rel) /\ frameOf (greference_of a t rel) == frameOf_aref a))
-  [SMTPat (frameOf (greference_of a t rel))]
-= ()
+let is_mm_greference_of _ _ _ = ()
 
-abstract
-let as_addr_greference_of
-  (a: aref)
-  (t: Type0)
-  (rel: preorder t)
-: Lemma
-  (requires (exists h . aref_live_at h a t rel))
-  (ensures ((exists h . aref_live_at h a t rel) /\ as_addr (greference_of a t rel) == aref_as_addr a))
-  [SMTPat (as_addr (greference_of a t rel))]
-= ()
+let unused_in_greference_of _ _ _ _ = ()
 
-abstract
-let is_mm_greference_of
-  (a: aref)
-  (t: Type0)
-  (rel: preorder t)
-: Lemma
-  (requires (exists h . aref_live_at h a t rel))
-  (ensures ((exists h . aref_live_at h a t rel) /\ is_mm (greference_of a t rel) == aref_is_mm a))
-  [SMTPat (is_mm (greference_of a t rel))]
-= ()
+let sel_reference_of _ _ _ _ _ = ()
 
-abstract
-let unused_in_greference_of
-  (a: aref)
-  (t: Type0)
-  (rel: preorder t)
-  (h: mem)
-: Lemma
-  (requires (exists h . aref_live_at h a t rel))
-  (ensures ((exists h . aref_live_at h a t rel) /\ (unused_in (greference_of a t rel) h <==> aref_unused_in a h)))
-  [SMTPat (unused_in (greference_of a t rel) h)]
-= ()
-
-abstract
-let sel_reference_of
-  (a: aref)
-  (v: Type0)
-  (rel: preorder v)
-  (h1 h2: mem)
-: Lemma
-  (requires (aref_live_at h1 a v rel /\ aref_live_at h2 a v rel))
-  (ensures (aref_live_at h2 a v rel /\ sel h1 (reference_of h2 a v rel) == sel h1 (greference_of a v rel)))
-  [SMTPat (sel h1 (reference_of h2 a v rel))]
-= ()
-
-abstract
-let upd_reference_of
-  (a: aref)
-  (v: Type0)
-  (rel: preorder v)
-  (h1 h2: mem)
-  (x: v)
-: Lemma
-  (requires (aref_live_at h1 a v rel /\ aref_live_at h2 a v rel))
-  (ensures (aref_live_at h1 a v rel /\ aref_live_at h2 a v rel /\ upd h1 (reference_of h2 a v rel) x == upd h1 (greference_of a v rel) x))
-  [SMTPat (upd h1 (reference_of h2 a v rel) x)]
-= ()
+let upd_reference_of _ _ _ _ _ _ = ()
