ulib/FStar.Monotonic.HyperStack.fsti
@@ -455,6 +455,10 @@ val eternal_disjoint_from_tip (h:mem{is_stack_region (get_tip h)})
                                      r `is_in` get_hmap h})
   :Lemma (disjoint (get_tip h) r)
 
+val above_tip_is_live (#a:Type) (#rel:preorder a) (m:mem) (x:mreference a rel)
+  :Lemma (requires (frameOf x `is_above` get_tip m))
+         (ensures  (frameOf x `is_in` get_hmap m))
+
 /////
 
 (****** Lemmas about equality of mem ******)
@@ -483,239 +487,108 @@ val lemma_next_addr_contained_refs_addr (_:unit)
 
 (* Definition and ghost decidable equality *)
 
-noeq abstract type aref: Type0 =
-| ARef:
-    (aref_region: rid) ->
-    (aref_aref: Heap.aref) ->
-    aref
+val aref: Type0
 
-abstract let dummy_aref : aref = ARef root Heap.dummy_aref
+val dummy_aref :aref
 
-abstract let aref_equal
-  (a1 a2: aref)
-: Ghost bool
-  (requires True)
-  (ensures (fun b -> b == true <==> a1 == a2))
-= a1.aref_region = a2.aref_region && Heap.aref_equal a1.aref_aref a2.aref_aref
+val aref_equal (a1 a2: aref)
+  :Ghost bool (requires True)
+              (ensures  (fun b -> b == true <==> a1 == a2))
 
 (* Introduction rule *)
 
-abstract let aref_of
-  (#t: Type)
-  (#rel: preorder t)
-  (r: mreference t rel)
-  : Tot aref
-  = ARef (frameOf r) (Heap.aref_of (as_ref r))
+val aref_of (#t: Type) (#rel: preorder t) (r: mreference t rel) :aref
 
 (* Operators lifted from reference *)
 
-abstract let frameOf_aref
-  (a: aref)
-: GTot rid
-= a.aref_region
+val frameOf_aref (a:aref) :GTot rid
 
-abstract let frameOf_aref_of
-  (#t: Type)
-  (#rel: preorder t)
-  (r: mreference t rel)
-: Lemma
-  (frameOf_aref (aref_of r) == frameOf r)
-  [SMTPat (frameOf_aref (aref_of r))]
-= ()
+val frameOf_aref_of (#t:Type) (#rel:preorder t) (r:mreference t rel)
+  :Lemma (frameOf_aref (aref_of r) == frameOf r)
+         [SMTPat (frameOf_aref (aref_of r))]
 
-abstract let aref_as_addr
-  (a: aref)
-: GTot (x: nat { x > 0 } )
-= Heap.addr_of_aref a.aref_aref
+val aref_as_addr (a:aref) :GTot pos
 
-abstract let aref_as_addr_aref_of
-  (#t: Type)
-  (#rel: preorder t)
-  (r: mreference t rel)
-: Lemma
-  (aref_as_addr (aref_of r) == as_addr r)
-  [SMTPat (aref_as_addr (aref_of r))]
-= Heap.addr_of_aref_of (as_ref r)
+val aref_as_addr_aref_of (#t:Type) (#rel:preorder t) (r:mreference t rel)
+  :Lemma (aref_as_addr (aref_of r) == as_addr r)
+         [SMTPat (aref_as_addr (aref_of r))]
 
-abstract let aref_is_mm
-  (r: aref)
-: GTot bool
-= Heap.aref_is_mm r.aref_aref
+val aref_is_mm (r:aref) :GTot bool
 
-abstract let is_mm_aref_of
-  (#t: Type)
-  (#rel: preorder t)
-  (r: mreference t rel)
-: Lemma
-  (aref_is_mm (aref_of r) == is_mm r)
-  [SMTPat (aref_is_mm (aref_of r))]
-= Heap.is_mm_aref_of (as_ref r)
+val is_mm_aref_of (#t:Type) (#rel:preorder t) (r:mreference t rel)
+  :Lemma (aref_is_mm (aref_of r) == is_mm r)
+         [SMTPat (aref_is_mm (aref_of r))]
 
-abstract let aref_unused_in
-  (a: aref)
-  (h: mem)
-: GTot Type0
-= ~ (live_region h a.aref_region) \/
-  Heap.aref_unused_in a.aref_aref (Map.sel h.h a.aref_region)
+val aref_unused_in (a:aref) (h:mem) :GTot Type0
 
-abstract let unused_in_aref_of
-  (#t: Type)
-  (#rel: preorder t)
-  (r: mreference t rel)
-  (h: mem)
-: Lemma
-  (aref_unused_in (aref_of r) h <==> unused_in r h)
-  [SMTPat (aref_unused_in (aref_of r) h)]
-= Heap.unused_in_aref_of (as_ref r) (Map.sel h.h (frameOf r))
+val unused_in_aref_of (#t:Type) (#rel:preorder t) (r:mreference t rel) (h:mem)
+  :Lemma (aref_unused_in (aref_of r) h <==> unused_in r h)
+         [SMTPat (aref_unused_in (aref_of r) h)]
 
-abstract
-val contains_aref_unused_in: #a:Type -> #rel: preorder a -> h:mem -> x:mreference a rel -> y:aref -> Lemma
-  (requires (contains h x /\ aref_unused_in y h))
-  (ensures  (frameOf x <> frameOf_aref y \/ as_addr x <> aref_as_addr y))
-  [SMTPat (contains h x); SMTPat (aref_unused_in y h)]
-let contains_aref_unused_in #a #rel h x y =
-  if frameOf x = frameOf_aref y
-  then
-    Heap.contains_aref_unused_in (Map.sel h.h (frameOf x)) (as_ref x) y.aref_aref
-  else ()
+val contains_aref_unused_in (#a:Type) (#rel:preorder a) (h:mem) (x:mreference a rel) (y:aref)
+  :Lemma (requires (contains h x /\ aref_unused_in y h))
+         (ensures  (frameOf x <> frameOf_aref y \/ as_addr x <> aref_as_addr y))
+         [SMTPat (contains h x); SMTPat (aref_unused_in y h)]
 
 (* Elimination rule *)
 
-abstract
-let aref_live_at
-  (h: mem)
-  (a: aref)
-  (v: Type)
-  (rel: preorder v)
-: GTot Type0
-= live_region h a.aref_region
-  /\ Heap.aref_live_at (Map.sel h.h a.aref_region) a.aref_aref v rel
+val aref_live_at (h:mem) (a:aref) (v:Type0) (rel:preorder v) :GTot Type0
 
-abstract
-let greference_of
-  (a: aref)
-  (v: Type)
-  (rel: preorder v)
-: Ghost (mreference v rel)
-  (requires (exists h . aref_live_at h a v rel))
-  (ensures (fun _ -> True))
-= MkRef a.aref_region (Heap.gref_of a.aref_aref v rel)
+val greference_of (a:aref) (v:Type0) (rel:preorder v)
+  :Ghost (mreference v rel) (requires (exists h . aref_live_at h a v rel))
+                            (ensures  (fun _ -> True))
 
-abstract
-let reference_of
-  (h: mem)
-  (a: aref)
-  (v: Type)
-  (rel: preorder v)
-: Pure (mreference v rel)
-  (requires (aref_live_at h a v rel))
-  (ensures (fun x -> aref_live_at h a v rel /\ frameOf x == frameOf_aref a /\ as_addr x == aref_as_addr a /\ is_mm x == aref_is_mm a))
-= MkRef a.aref_region (Heap.ref_of (Map.sel h.h a.aref_region) a.aref_aref v rel)
+val reference_of (h:mem) (a:aref) (v:Type0) (rel:preorder v)
+  :Pure (mreference v rel) (requires (aref_live_at h a v rel))
+                           (ensures  (fun x -> aref_live_at h a v rel /\ frameOf x == frameOf_aref a /\
+			                    as_addr x == aref_as_addr a /\ is_mm x == aref_is_mm a))
 
-abstract
-let aref_live_at_aref_of
-  (h: mem)
-  (#t: Type0)
-  (#rel: preorder t)
-  (r: mreference t rel)
-: Lemma
-  (aref_live_at h (aref_of r) t rel <==> contains h r)
-  [SMTPat (aref_live_at h (aref_of r) t rel)]
-= ()
+val aref_live_at_aref_of (h:mem) (#t:Type0) (#rel:preorder t) (r:mreference t rel)
+  :Lemma (aref_live_at h (aref_of r) t rel <==> contains h r)
+         [SMTPat (aref_live_at h (aref_of r) t rel)]
 
-abstract
-let contains_greference_of
-  (h: mem)
-  (a: aref)
-  (t: Type0)
-  (rel: preorder t)
-: Lemma
-  (requires (exists h' . aref_live_at h' a t rel))
-  (ensures ((exists h' . aref_live_at h' a t rel) /\ (contains h (greference_of a t rel) <==> aref_live_at h a t rel)))
-  [SMTPatOr [
-    [SMTPat (contains h (greference_of a t rel))];
-    [SMTPat (aref_live_at h a t rel)];
-  ]]
-= ()
+val contains_greference_of (h:mem) (a:aref) (t:Type0) (rel:preorder t)
+  :Lemma (requires (exists h' . aref_live_at h' a t rel))
+         (ensures  ((exists h' . aref_live_at h' a t rel) /\ (contains h (greference_of a t rel) <==> aref_live_at h a t rel)))
+         [SMTPatOr [
+             [SMTPat (contains h (greference_of a t rel))];
+             [SMTPat (aref_live_at h a t rel)];
+         ]]
 
-abstract
-let aref_of_greference_of
-  (a: aref)
-  (v: Type0)
-  (rel: preorder v)
-: Lemma
-  (requires (exists h' . aref_live_at h' a v rel))
-  (ensures ((exists h' . aref_live_at h' a v rel) /\ aref_of (greference_of a v rel) == a))
-  [SMTPat (aref_of (greference_of a v rel))]
-= ()
+val aref_of_greference_of (a:aref) (v:Type0) (rel:preorder v)
+  :Lemma (requires (exists h' . aref_live_at h' a v rel))
+         (ensures  ((exists h' . aref_live_at h' a v rel) /\ aref_of (greference_of a v rel) == a))
+         [SMTPat (aref_of (greference_of a v rel))]
 
 (* Operators lowered to rref *)
 
-abstract let frameOf_greference_of
-  (a: aref)
-  (t: Type)
-  (rel: preorder t)
-: Lemma
-  (requires (exists h . aref_live_at h a t rel))
-  (ensures ((exists h . aref_live_at h a t rel) /\ frameOf (greference_of a t rel) == frameOf_aref a))
-  [SMTPat (frameOf (greference_of a t rel))]
-= ()
+val frameOf_greference_of (a:aref) (t:Type0) (rel:preorder t)
+  :Lemma (requires (exists h . aref_live_at h a t rel))
+         (ensures  ((exists h . aref_live_at h a t rel) /\ frameOf (greference_of a t rel) == frameOf_aref a))
+         [SMTPat (frameOf (greference_of a t rel))]
 
-abstract
-let as_addr_greference_of
-  (a: aref)
-  (t: Type0)
-  (rel: preorder t)
-: Lemma
-  (requires (exists h . aref_live_at h a t rel))
-  (ensures ((exists h . aref_live_at h a t rel) /\ as_addr (greference_of a t rel) == aref_as_addr a))
-  [SMTPat (as_addr (greference_of a t rel))]
-= ()
+val as_addr_greference_of (a:aref) (t:Type0) (rel:preorder t)
+  :Lemma (requires (exists h . aref_live_at h a t rel))
+         (ensures  ((exists h . aref_live_at h a t rel) /\ as_addr (greference_of a t rel) == aref_as_addr a))
+         [SMTPat (as_addr (greference_of a t rel))]
 
-abstract
-let is_mm_greference_of
-  (a: aref)
-  (t: Type0)
-  (rel: preorder t)
-: Lemma
-  (requires (exists h . aref_live_at h a t rel))
-  (ensures ((exists h . aref_live_at h a t rel) /\ is_mm (greference_of a t rel) == aref_is_mm a))
-  [SMTPat (is_mm (greference_of a t rel))]
-= ()
+val is_mm_greference_of (a:aref) (t:Type0) (rel:preorder t)
+  :Lemma (requires (exists h . aref_live_at h a t rel))
+         (ensures  ((exists h . aref_live_at h a t rel) /\ is_mm (greference_of a t rel) == aref_is_mm a))
+         [SMTPat (is_mm (greference_of a t rel))]
 
-abstract
-let unused_in_greference_of
-  (a: aref)
-  (t: Type0)
-  (rel: preorder t)
-  (h: mem)
-: Lemma
-  (requires (exists h . aref_live_at h a t rel))
-  (ensures ((exists h . aref_live_at h a t rel) /\ (unused_in (greference_of a t rel) h <==> aref_unused_in a h)))
-  [SMTPat (unused_in (greference_of a t rel) h)]
-= ()
+val unused_in_greference_of (a:aref) (t:Type0) (rel:preorder t) (h:mem)
+  :Lemma (requires (exists h . aref_live_at h a t rel))
+         (ensures  ((exists h . aref_live_at h a t rel) /\ (unused_in (greference_of a t rel) h <==> aref_unused_in a h)))
+         [SMTPat (unused_in (greference_of a t rel) h)]
 
-abstract
-let sel_reference_of
-  (a: aref)
-  (v: Type0)
-  (rel: preorder v)
-  (h1 h2: mem)
-: Lemma
-  (requires (aref_live_at h1 a v rel /\ aref_live_at h2 a v rel))
-  (ensures (aref_live_at h2 a v rel /\ sel h1 (reference_of h2 a v rel) == sel h1 (greference_of a v rel)))
-  [SMTPat (sel h1 (reference_of h2 a v rel))]
-= ()
+val sel_reference_of (a:aref) (v:Type0) (rel:preorder v) (h1 h2: mem)
+  :Lemma (requires (aref_live_at h1 a v rel /\ aref_live_at h2 a v rel))
+         (ensures  (aref_live_at h2 a v rel /\ sel h1 (reference_of h2 a v rel) == sel h1 (greference_of a v rel)))
+         [SMTPat (sel h1 (reference_of h2 a v rel))]
 
-abstract
-let upd_reference_of
-  (a: aref)
-  (v: Type0)
-  (rel: preorder v)
-  (h1 h2: mem)
-  (x: v)
-: Lemma
-  (requires (aref_live_at h1 a v rel /\ aref_live_at h2 a v rel))
-  (ensures (aref_live_at h1 a v rel /\ aref_live_at h2 a v rel /\ upd h1 (reference_of h2 a v rel) x == upd h1 (greference_of a v rel) x))
-  [SMTPat (upd h1 (reference_of h2 a v rel) x)]
-= ()
+val upd_reference_of (a:aref) (v:Type0) (rel:preorder v) (h1 h2:mem) (x:v)
+  :Lemma (requires (aref_live_at h1 a v rel /\ aref_live_at h2 a v rel))
+         (ensures  (aref_live_at h1 a v rel /\ aref_live_at h2 a v rel /\
+	            upd h1 (reference_of h2 a v rel) x == upd h1 (greference_of a v rel) x))
+         [SMTPat (upd h1 (reference_of h2 a v rel) x)]
